examples/cannon/CannonA.v
@@ -1,6 +1,6 @@
 Require Import Coqlib ITreelib sflib.
 Require Import ImpPrelude.
-Require Import Events STS.
+Require Import Events.
 Require Import Behavior.
 Require Import SMod HMod.
 Require Import Skeleton.
@@ -13,13 +13,14 @@ Set Implicit Arguments.
 
 Module CannonA.
 Section A.
-  Context `{_W: CtxWD.t}.
-  Context `{_A: CannonAR.t (Γ:=Γ)}.
+  Import CannonAS.
+  Context `{!Inv.t Σ Γ α β τ, !G Γ}.
+  Local Notation iProp := (iProp Σ).
 
   Definition scopes := ["Cannon"].
   Definition v_lv := "Cannon" ↯ "lv".
 
-  Definition fire: list val -> itree smodE Z :=
+  Definition fire: list val -> itree hmodE Z :=
     fun _ =>
       let r := 1%Z in
       _ <- trigger (@IO _ void "print" [r]↑);;
@@ -45,7 +46,7 @@ Section A.
   |}.
 
   Definition InitCond : Sk.t -> iProp :=
-    fun _ => (OwnM CannonAS.Ready)%I.
+    fun _ => Ready%I.
 
   Variable ginv: Sk.t -> invspec.
   Variable GlobalStb: Sk.t -> gname -> option fspec.
